Generalize kinds of sum cases

src/lowparse/LowParseExample.Aux.fst
@@ -10,7 +10,7 @@ module L = FStar.List.Tot
 noeq
 type t =
   | A of (U8.t * U8.t)
-  | B of U16.t
+  | B of (x: U16.t { U16.v x > 0 } )
 
 type cases =
   | Case_A
@@ -58,7 +58,7 @@ let synth_case_A_inj () : Lemma
 = ()
 
 inline_for_extraction
-let synth_case_B (z: (U16.t)) : Tot (LP.sum_cases t_sum Case_B) =
+let synth_case_B (z: (U16.t) { U16.v z > 0 } ) : Tot (LP.sum_cases t_sum Case_B) =
   [@inline_let]
   let res : t = B z in
   [@inline_let]
@@ -70,24 +70,36 @@ let synth_case_B (z: (U16.t)) : Tot (LP.sum_cases t_sum Case_B) =
 let synth_case_B_inj () : Lemma
   (LP.synth_injective synth_case_B)
 = ()
-  
-let parse_cases
-  (x: LP.sum_key t_sum)
-: Tot (LP.parser LP.parse_u16_kind  (LP.sum_cases t_sum x))
-= match x with
-  | Case_A ->
+
+let parse_case_B_filter
+  (x: U16.t)
+: GTot bool
+= U16.v x > 0
+
+let parse_case_A : LP.parser _ (LP.sum_cases t_sum Case_A) =
     synth_case_A_inj ();
     LP.parse_synth (LP.parse_u8 `LP.nondep_then` LP.parse_u8) synth_case_A
-  | Case_B ->
+
+let parse_case_B : LP.parser _ (LP.sum_cases t_sum Case_B) =
     synth_case_B_inj ();
-    LP.parse_synth LP.parse_u16 synth_case_B
+    LP.parse_synth (LP.parse_filter LP.parse_u16 parse_case_B_filter) synth_case_B
+
+let parse_cases'
+  (x: LP.sum_key t_sum)
+: Tot (k: LP.parser_kind & LP.parser k  (LP.sum_cases t_sum x))
+= match x with
+  | Case_A -> (| _, parse_case_A |)
+  | Case_B -> (| _, parse_case_B |)
+
+let parse_cases :
+  (x: LP.sum_key t_sum) ->
+  Tot (LP.parser _ (LP.sum_cases t_sum x))
+= LP.parse_sum_cases t_sum parse_cases'
 
 inline_for_extraction
-let parse32_cases
-  (x: LP.sum_key t_sum)
-: Tot (LP.parser32 (parse_cases x))
-= match x with
-  | Case_A ->
+let parse32_cases_A
+: (LP.parser32 parse_case_A)
+=
     [@inline_let]
     let _ = synth_case_A_inj () in
     LP.parse32_synth
@@ -96,17 +108,40 @@ let parse32_cases
       (fun x -> synth_case_A x)
       (LP.parse32_nondep_then LP.parse32_u8 LP.parse32_u8)
       ()
-  | Case_B ->
+
+inline_for_extraction
+let parse32_cases_B
+: (LP.parser32 parse_case_B)
+=
     [@inline_let]
     let _ = synth_case_B_inj () in
     LP.parse32_synth
       _
       synth_case_B
-      (fun x -> synth_case_B x)
-      LP.parse32_u16
+      (fun (x: U16.t { parse_case_B_filter x == true } ) -> synth_case_B x)
+      (LP.parse32_filter LP.parse32_u16 parse_case_B_filter (fun x -> U16.gt x 0us))
       ()
 
-let parse_t : LP.parser _ t =
+inline_for_extraction
+let parse32_cases'
+  (x: LP.sum_key t_sum)
+: Tot (LP.parser32 (dsnd (parse_cases' x)))
+= match x with
+  | Case_A -> parse32_cases_A
+  | Case_B -> parse32_cases_B
+
+inline_for_extraction
+let parse32_cases
+: (x: LP.sum_key t_sum) ->
+  Tot (LP.parser32 (parse_cases x))
+= LP.parse32_sum_cases t_sum parse_cases' parse32_cases'
+
+let parse_t_kind : LP.parser_kind =
+  LP.and_then_kind
+    (LP.parse_filter_kind LP.parse_u8_kind)
+    (LP.weaken_parse_cases_kind t_sum parse_cases')
+
+let parse_t : LP.parser parse_t_kind t =
   LP.parse_sum t_sum LP.parse_u8 parse_cases
 
 inline_for_extraction
@@ -142,7 +177,7 @@ let cases_of_t_B (x: t) : Lemma
 = ()
 
 inline_for_extraction
-let synth_case_B_inv (z: LP.sum_cases t_sum Case_B) : Tot (z: U16.t) =
+let synth_case_B_inv (z: LP.sum_cases t_sum Case_B) : Tot (z: U16.t { UInt16.v z > 0 } ) =
   [@inline_let]
   let z' : t = z in
   let _ = cases_of_t_B z' in
@@ -153,46 +188,51 @@ let synth_case_B_inv_correct () : Lemma
   (LP.synth_inverse synth_case_B synth_case_B_inv)
 = ()
 
-let serialize_cases
-  (x: LP.sum_key t_sum)
-: Tot (LP.serializer (parse_cases x))
-= match x with
-  | Case_A ->
+let serialize_case_A
+: LP.serializer parse_case_A
+= 
     synth_case_A_inj ();
     synth_case_A_inv_correct ();
-    LP.serialize_ext'
-      _
       (LP.serialize_synth
-        _
+        (LP.nondep_then LP.parse_u8 LP.parse_u8)
         synth_case_A
-        (LP.serialize_nondep_then _ LP.serialize_u8 () _ LP.serialize_u8)
+        (LP.serialize_nondep_then LP.parse_u8 LP.serialize_u8 () LP.parse_u8 LP.serialize_u8)
         synth_case_A_inv
         ()
       )
-      (parse_cases x)
-  | Case_B ->
+
+let serialize_case_B
+: LP.serializer parse_case_B
+= 
     synth_case_B_inj ();
     synth_case_B_inv_correct ();
-    LP.serialize_ext'
-      _
       (LP.serialize_synth
-        LP.parse_u16
+        (LP.parse_filter LP.parse_u16 parse_case_B_filter)
         synth_case_B
-        LP.serialize_u16
+        (LP.serialize_filter #_ #_ #LP.parse_u16 LP.serialize_u16 parse_case_B_filter)
         synth_case_B_inv
         ()
       )
-      (parse_cases x)
+
+let serialize_cases'
+  (x: LP.sum_key t_sum)
+: Tot (LP.serializer (dsnd (parse_cases' x)))
+= match x with
+  | Case_A -> serialize_case_A
+  | Case_B -> serialize_case_B
+
+let serialize_cases
+: (x: LP.sum_key t_sum) ->
+  Tot (LP.serializer (parse_cases x))
+= LP.serialize_sum_cases t_sum parse_cases' serialize_cases'
 
 let serialize_t : LP.serializer parse_t =
   LP.serialize_sum t_sum LP.serialize_u8 serialize_cases
 
 inline_for_extraction
-let serialize32_cases
-  (x: LP.sum_key t_sum)
-: Tot (LP.serializer32 (serialize_cases x))
-= match x with
-  | Case_A ->
+let serialize32_case_A
+: LP.serializer32 (serialize_case_A)
+= 
       [@inline_let]
       let _ = synth_case_A_inj () in
       [@inline_let]
@@ -205,62 +245,138 @@ let serialize32_cases
         synth_case_A_inv
         (fun x -> synth_case_A_inv x)
         ()
-  | Case_B ->
+
+inline_for_extraction
+let serialize32_case_B
+: LP.serializer32 (serialize_case_B)
+=
       [@inline_let]
       let _ = synth_case_B_inj () in
       [@inline_let]
       let _ = synth_case_B_inv_correct () in
       LP.serialize32_synth
-        LP.parse_u16
+        (LP.parse_filter LP.parse_u16 parse_case_B_filter)
         synth_case_B
-        LP.serialize_u16
-        LP.serialize32_u16
+        (LP.serialize_filter LP.serialize_u16 parse_case_B_filter)
+        (LP.serialize32_filter LP.serialize32_u16 parse_case_B_filter)
         synth_case_B_inv
         (fun x -> synth_case_B_inv x)
         ()
 
 inline_for_extraction
-let serialize32_t : LP.serializer32 serialize_t =
-  FStar.Tactics.synth_by_tactic (
-    LP.serialize32_sum_tac
-      t_sum
-      #_
-      #LP.serialize_u8
+let serialize32_cases'
+  (x: LP.sum_key t_sum)
+: Tot (LP.serializer32 (serialize_cases' x))
+= match x with
+  | Case_A -> serialize32_case_A
+  | Case_B -> serialize32_case_B
+
+inline_for_extraction
+let serialize32_cases
+: (x: LP.sum_key t_sum) ->
+  Tot (LP.serializer32 (serialize_cases x))
+= LP.serialize32_sum_cases
+    t_sum
+    parse_cases'
+    serialize_cases'
+    serialize32_cases'
+
+inline_for_extraction
+let t_sum_destr
+: LP.sum_destr LP.bytes32 t_sum
+= let open FStar.Tactics in
+  synth_by_tactic
+  (u <-- LP.sum_destr_tac LP.bytes32 t_sum ;
+  exact_guard (return u))
+
+inline_for_extraction
+let serialize32_t_sum_enum
+: LP.serializer32 (LP.serialize_enum_key _ LP.serialize_u8 (LP.sum_enum t_sum))
+= FStar.Tactics.synth_by_tactic (
+    LP.serialize32_enum_key_gen_tac
+      #_ #_ #_ #LP.parse_u8 #LP.serialize_u8
       LP.serialize32_u8
-      #_
-      serialize32_cases
-      ()
-      (fun x -> cases_of_t x)
-      serialize_t
+      (LP.sum_enum t_sum)
+      (LP.serialize_enum_key _ LP.serialize_u8 (LP.sum_enum t_sum))
       ()
   )
 
+inline_for_extraction
+let serialize32_t : LP.serializer32 serialize_t =
+  [@inline_let]
+  let _ = assert_norm (
+    LP.serializer32_sum_gen_precond
+      LP.parse_u8_kind
+      (LP.weaken_parse_cases_kind t_sum parse_cases')
+  )
+  in
+  LP.serialize32_sum_gen
+    t_sum
+    LP.serialize_u8
+    serialize32_cases
+    ()
+    (fun x -> cases_of_t x)
+    serialize_t
+    ()
+    serialize32_t_sum_enum
+    t_sum_destr
+
+let parse_t_array_precond () : Lemma
+  (LP.fldata_array_precond
+      parse_t
+      54
+      18
+    == true)
+= assert_norm (
+    LP.fldata_array_precond
+      parse_t
+      54
+      18
+    == true   
+  )
+
 let parse_t_array : LP.parser _ (LP.array t 18) =
+  parse_t_array_precond ();
   LP.parse_array serialize_t 54 18
 
 inline_for_extraction
 let parse32_t_array : LP.parser32 parse_t_array =
+  [@inline_let]
+  let _ = parse_t_array_precond () in
   LP.parse32_array serialize_t parse32_t 54 54ul 18 ()
 
 let serialize_t_array : LP.serializer parse_t_array =
+  parse_t_array_precond ();
   LP.serialize_array serialize_t 54 18 ()
 
 inline_for_extraction
 let serialize32_t_array : LP.serializer32 serialize_t_array =
+  [@inline_let]
+  let _ = parse_t_array_precond () in
   LP.serialize32_array #_ #_ #parse_t #serialize_t serialize32_t 54 18 ()
 
 // NOTE: in this example, byte-size bounds do not need to exactly match element-count bounds (which would be 15 and 21 respectively)
 
+let parse_t_vlarray_precond () : Lemma
+  (LP.vldata_vlarray_precond 13 22 parse_t 5 7 == true)
+= assert_norm (LP.vldata_vlarray_precond 13 22 parse_t 5 7 == true)
+
 let parse_t_vlarray : LP.parser _ (LP.vlarray t 5 7) =
+  parse_t_vlarray_precond ();
   LP.parse_vlarray 13 22 serialize_t 5 7 ()
 
 inline_for_extraction
 let parse32_t_vlarray : LP.parser32 parse_t_vlarray =
+  [@inline_let]
+  let _ = parse_t_vlarray_precond () in
   LP.parse32_vlarray 13 13ul 22 22ul serialize_t parse32_t 5 7 ()
 
 let serialize_t_vlarray : LP.serializer parse_t_vlarray =
+  parse_t_vlarray_precond ();
   LP.serialize_vlarray 13 22 serialize_t 5 7 ()
 
 inline_for_extraction
 let serialize32_t_vlarray : LP.serializer32 serialize_t_vlarray =
+  [@inline_let]
+  let _ = parse_t_vlarray_precond () in
   LP.serialize32_vlarray 13 22 #_ #_ #parse_t #serialize_t serialize32_t 5 7 ()
